add metrics to WeakestPrecondition
all WeakestPreconditionProperties proofs are appropriately adapted, but
nowhere they're used has been updated (so this commit doesn't compile)

bedrock2/src/bedrock2/WeakestPrecondition.v
@@ -1,134 +1,169 @@
 Require Import coqutil.Macros.subst coqutil.Macros.unique bedrock2.Notations coqutil.Map.Interface coqutil.Map.OfListWord.
 Require Import Coq.ZArith.BinIntDef coqutil.Word.Interface.
 Require Import coqutil.dlet bedrock2.Syntax bedrock2.Semantics.
+Require Import bedrock2.MetricLogging.
 
 Section WeakestPrecondition.
   Context {p : unique! Semantics.parameters}.
 
-  Definition literal v (post : word -> Prop) : Prop :=
-    dlet! v := word.of_Z v in post v.
-  Definition get (l : locals) (x : String.string) (post : word -> Prop) : Prop :=
-    bind_ex_Some v <- map.get l x; post v.
-  Definition load s m a (post : _ -> Prop) : Prop :=
-    bind_ex_Some v <- load s m a; post v.
+  Local Notation metrics := MetricLog.
+
+  Definition literal v mc (post : (word * metrics) -> Prop) : Prop :=
+    dlet! v := word.of_Z v in post (v, addMetricInstructions 8 (addMetricLoads 8 mc)).
+  Definition get (l : locals) (x : String.string) mc (post : (word * metrics) -> Prop) : Prop :=
+    bind_ex_Some v <- map.get l x; post (v, addMetricInstructions 1 (addMetricLoads 2 mc)).
+  Definition load s m a mc (post : (word * metrics) -> Prop) : Prop :=
+    bind_ex_Some v <- load s m a; post (v, addMetricInstructions 1 (addMetricLoads 2 mc)).
   Definition store sz m a v post :=
     bind_ex_Some m <- store sz m a v; post m.
 
   Section WithMemAndLocals.
     Context (m : mem) (l : locals).
-    Definition expr_body rec (e : Syntax.expr) (post : word -> Prop) : Prop :=
+
+    (* with execution time verification; just-correctness-oriented version below *)
+    Definition expr_body (rec : _->_->(word*metrics->Prop)->Prop) (e : Syntax.expr) (mc : metrics) (post : word * metrics -> Prop) : Prop :=
       match e with
       | expr.literal v =>
-        literal v post
+        literal v mc post
       | expr.var x =>
-        get l x post
+        get l x mc post
       | expr.op op e1 e2 =>
-        rec e1 (fun v1 =>
-        rec e2 (fun v2 =>
-        post (interp_binop op v1 v2)))
+        rec e1 mc (fun '(v1, mc') =>
+        rec e2 mc' (fun '(v2, mc'') =>
+        post (interp_binop op v1 v2, addMetricInstructions 2 (addMetricLoads 2 mc''))))
       | expr.load s e =>
-        rec e (fun a =>
-        load s m a post)
+        rec e mc (fun '(a, mc') =>
+        load s m a mc' post)
       | expr.inlinetable s t e =>
-        rec e (fun a =>
-        load s (map.of_list_word t) a post)
+        rec e mc (fun '(a, mc') =>
+        load s (map.of_list_word t) a (addMetricInstructions 2
+                                      (addMetricLoads 2
+                                      (addMetricJumps 1 mc'))) post)
     end.
+
+    (*Definition expr_body rec (e : Syntax.expr) (post : word -> Prop) : Prop :=*)
+    (*  match e with*)
+    (*  | expr.literal v =>*)
+    (*    literal v post*)
+    (*  | expr.var x =>*)
+    (*    get l x post*)
+    (*  | expr.op op e1 e2 =>*)
+    (*    rec e1 (fun v1 =>*)
+    (*    rec e2 (fun v2 =>*)
+    (*    post (interp_binop op v1 v2)))*)
+    (*  | expr.load s e =>*)
+    (*    rec e (fun a =>*)
+    (*    load s m a post)*)
+    (*  | expr.inlinetable s t e =>*)
+    (*    rec e (fun a =>*)
+    (*    load s (map.of_list_word t) a post)*)
+    (*end.*)
+
     Fixpoint expr e := expr_body expr e.
   End WithMemAndLocals.
 
   Section WithF.
-    Context {A B} (f: A -> (B -> Prop) -> Prop).
-    Definition list_map_body rec (xs : list A) (post : list B -> Prop) : Prop :=
+    Context {A B} (f: A -> metrics -> (B * metrics -> Prop) -> Prop).
+    Definition list_map_body rec (xs : list A) (mc : metrics) (post : list B * metrics -> Prop) : Prop :=
       match xs with
-      | nil => post nil
+      | nil => post (nil, mc)
       | cons x xs' =>
-        f x (fun y =>
-        rec xs' (fun ys' =>
-        post (cons y ys')))
+        f x mc (fun '(y, mc') =>
+        rec xs' mc' (fun '(ys', mc'') =>
+        post (cons y ys', mc'')))
       end.
     Fixpoint list_map xs := list_map_body list_map xs.
   End WithF.
 
   Section WithFunctions.
-    Context (call : String.string -> trace -> mem -> list word -> (trace -> mem -> list word -> Prop) -> Prop).
-    Definition dexpr m l e v := expr m l e (eq v).
-    Definition dexprs m l es vs := list_map (expr m l) es (eq vs).
-    Definition cmd_body (rec:_->_->_->_->_->Prop) (c : cmd) (t : trace) (m : mem) (l : locals)
-             (post : trace -> mem -> locals -> Prop) : Prop :=
+    Context (call : String.string -> trace -> mem -> list word -> metrics -> (trace -> mem -> list word -> metrics -> Prop) -> Prop).
+    Definition dexpr m l e mc vmc := expr m l e mc (eq vmc).
+    Definition dexprs m l es mc vmcs := list_map (expr m l) es mc (eq vmcs).
+    Definition cmd_body (rec:_->_->_->_->_->_->Prop) (c : cmd) (t : trace) (m : mem) (l : locals) (mc : metrics)
+             (post : trace -> mem -> locals -> metrics -> Prop) : Prop :=
       (* give value of each pure expression when stating its subproof *)
       match c with
-      | cmd.skip => post t m l
+      | cmd.skip => post t m l mc
       | cmd.set x ev =>
-        bind_ex v <- dexpr m l ev;
+        bind_ex_pair (v, mc') <- dexpr m l ev mc;
         dlet! l := map.put l x v in
-        post t m l
+        post t m l (addMetricInstructions 1 (addMetricLoads 1 mc'))
       | cmd.unset x =>
         dlet! l := map.remove l x in
-        post t m l
+        post t m l mc
       | cmd.store sz ea ev =>
-        bind_ex a <- dexpr m l ea;
-        bind_ex v <- dexpr m l ev;
+        bind_ex_pair (a, mc') <- dexpr m l ea mc;
+        bind_ex_pair (v, mc'') <- dexpr m l ev mc';
         store sz m a v (fun m =>
-        post t m l)
+        post t m l (addMetricInstructions 1 (addMetricLoads 1 (addMetricStores 1 mc''))))
       | cmd.stackalloc x n c =>
         Z.modulo n (bytes_per_word width) = 0 /\
         forall a mStack mCombined,
           anybytes a n mStack -> map.split mCombined m mStack ->
           dlet! l := map.put l x a in
-          rec c t mCombined l (fun t' mCombined' l' =>
+          rec c t mCombined l (addMetricInstructions 1 (addMetricLoads 1 mc))
+          (fun t' mCombined' l' mc' =>
           exists m' mStack',
           anybytes a n mStack' /\ map.split mCombined' m' mStack' /\
-          post t' m' l')
+          post t' m' l' mc')
       | cmd.cond br ct cf =>
-        bind_ex v <- dexpr m l br;
-        (word.unsigned v <> 0%Z -> rec ct t m l post) /\
-        (word.unsigned v = 0%Z -> rec cf t m l post)
+        bind_ex_pair (v, mc') <- dexpr m l br mc;
+        dlet! mc'' := addMetricInstructions 2 (addMetricLoads 2 (addMetricJumps 1 mc')) in
+        (word.unsigned v <> 0%Z -> rec ct t m l mc'' post) /\
+        (word.unsigned v = 0%Z -> rec cf t m l mc'' post)
       | cmd.seq c1 c2 =>
-        rec c1 t m l (fun t m l => rec c2 t m l post)
+        rec c1 t m l mc (fun t m l mc => rec c2 t m l mc post)
       | cmd.while e c =>
-        exists measure (lt:measure->measure->Prop) (inv:measure->trace->mem->locals->Prop),
+        exists measure (lt:measure->measure->Prop) (inv:measure->trace->mem->locals->metrics->Prop),
         Coq.Init.Wf.well_founded lt /\
-        (exists v, inv v t m l) /\
-        (forall v t m l, inv v t m l ->
-          bind_ex b <- dexpr m l e;
-          (word.unsigned b <> 0%Z -> rec c t m l (fun t' m l =>
-            exists v', inv v' t' m l /\ lt v' v)) /\
-          (word.unsigned b = 0%Z -> post t m l))
+        (exists v, inv v t m l mc) /\
+        (forall v t m l mc, inv v t m l mc ->
+          bind_ex_pair (b, mc') <- dexpr m l e mc;
+          (word.unsigned b <> 0%Z -> rec c t m l mc' (fun t' m' l' mc'' =>
+            exists v', inv v' t' m' l' (addMetricInstructions 2
+                                       (addMetricLoads 2
+                                       (addMetricJumps 1 mc''))) /\ lt v' v)) /\
+          (word.unsigned b = 0%Z -> post t m l (addMetricInstructions 1
+                                               (addMetricLoads 1
+                                               (addMetricJumps 1 mc')))))
       | cmd.call binds fname arges =>
-        bind_ex args <- dexprs m l arges;
-        call fname t m args (fun t m rets =>
+        bind_ex_pair (args, mc') <- dexprs m l arges mc;
+        call fname t m args mc' (fun t m rets mc'' =>
           bind_ex_Some l <- map.putmany_of_list_zip binds rets l;
-          post t m l)
+          post t m l mc'')
       | cmd.interact binds action arges =>
-        bind_ex args <- dexprs m l arges;
+        bind_ex_pair (args, mc') <- dexprs m l arges mc;
         exists mKeep mGive, map.split m mKeep mGive /\
         ext_spec t mGive action args (fun mReceive rets =>
           bind_ex_Some l' <- map.putmany_of_list_zip binds rets l;
           forall m', map.split m' mKeep mReceive ->
-          post (cons ((mGive, action, args), (mReceive, rets)) t) m' l')
+          post (cons ((mGive, action, args), (mReceive, rets)) t) m' l' (addMetricInstructions 1
+                                                                        (addMetricStores 1
+                                                                        (addMetricLoads 2 mc'))))
       end.
     Fixpoint cmd c := cmd_body cmd c.
   End WithFunctions.
 
-  Definition func call '(innames, outnames, c) (t : trace) (m : mem) (args : list word) (post : trace -> mem -> list word -> Prop) :=
+  Definition func call '(innames, outnames, c) (t : trace) (m : mem) (args : list word) (mc : metrics) (post : trace -> mem -> list word -> metrics -> Prop) :=
       bind_ex_Some l <- map.of_list_zip innames args;
-      cmd call c t m l (fun t m l =>
-        list_map (get l) outnames (fun rets =>
-        post t m rets)).
+      cmd call c t m l mc (fun t m l mc =>
+        (* this list_map is only used proof-side and not actually executed in the program, so ignore the new metrics *)
+        list_map (get l) outnames mc (fun '(rets, _) =>
+        post t m rets mc)).
 
   Definition call_body rec (functions : list (String.string * (list String.string * list String.string * cmd.cmd)))
-                (fname : String.string) (t : trace) (m : mem) (args : list word)
-                (post : trace -> mem -> list word -> Prop) : Prop :=
+                (fname : String.string) (t : trace) (m : mem) (args : list word) (mc : metrics)
+                (post : trace -> mem -> list word -> metrics -> Prop) : Prop :=
     match functions with
     | nil => False
     | cons (f, decl) functions =>
       if String.eqb f fname
-      then func (rec functions) decl t m args post
-      else rec functions fname t m args post
+      then func (rec functions) decl t m args mc post
+      else rec functions fname t m args mc post
     end.
   Fixpoint call functions := call_body call functions.
 
-  Definition program funcs main t m l post : Prop := cmd (call funcs) main t m l post.
+  Definition program funcs main t m l mc post : Prop := cmd (call funcs) main t m l mc post.
 End WeakestPrecondition.
 
 Ltac unfold1_cmd e :=
